extraction/theories/ESubstitution.v
@@ -10,7 +10,6 @@ Local Open Scope list_scope.
 Set Asymmetric Patterns.
 Import MonadNotation.
 
-
 Existing Instance config.default_checker_flags.
 Module PA := PCUICAst.
 Module P := PCUICWcbvEval.
@@ -19,162 +18,158 @@ Module P := PCUICWcbvEval.
 
 (** ** Weakening *)
 
-Lemma extract_weakening `{Fuel} (Σ : PCUICAst.global_context) (Γ Γ' : PCUICAst.context) (t T : PCUICAst.term) t' :
+Lemma extract_weakening (Σ : PCUICAst.global_context) (Γ Γ' : PCUICAst.context) (t T : PCUICAst.term) :
     wf Σ ->
     wf_local Σ (Γ ,,, Γ') ->
     Σ;;; Γ |- t : T ->
-    extract Σ Γ t = Checked t' -> extract Σ (Γ ,,, Γ') (PCUICLiftSubst.lift #|Γ'| 0 t) = Checked (lift #|Γ'| 0 t').
+    extract Σ (Γ ,,, Γ') (PCUICLiftSubst.lift #|Γ'| 0 t) = lift #|Γ'| 0 (extract Σ Γ t).
 Admitted.
 
-(** ** Substitution *)
+(* (** ** Substitution *) *)
   
-Lemma is_arity_subst `{Fuel} Σ Γ Γ' Δ a s :
-  wf Σ -> subslet Σ Γ s Γ' ->
-  (* Σ ;;; Γ ,,, Γ' ,,, Δ |- a : T -> *)
-  wf_local Σ (Γ ,,, subst_context s 0 Δ) ->
-  is_arity Σ (Γ ,,, Γ' ,,, Δ) _ a = is_arity Σ (Γ ,,, subst_context s 0 Δ) _ (PCUICLiftSubst.subst s #|Δ| a). 
-Proof.
-Admitted.
+(* Lemma is_arity_subst Σ Γ Γ' Δ a s : *)
+(*   wf Σ -> subslet Σ Γ s Γ' -> *)
+(*   (* Σ ;;; Γ ,,, Γ' ,,, Δ |- a : T -> *) *)
+(*   wf_local Σ (Γ ,,, subst_context s 0 Δ) -> *)
+(*   is_arity Σ (Γ ,,, Γ' ,,, Δ) _ a = is_arity Σ (Γ ,,, subst_context s 0 Δ) _ (PCUICLiftSubst.subst s #|Δ| a).  *)
+(* Proof. *)
+(* Admitted. *)
 
-(* this is probably too strict, a might also be an algebraic universe *)
-Lemma type_of_subst `{Fuel} Σ Γ Γ' Δ a T s T' :
+(* (* this is probably too strict, a might also be an algebraic universe *) *)
+(* Lemma type_of_subst Σ Γ Γ' Δ a T s T' : *)
+(*   wf Σ -> subslet Σ Γ s Γ' -> *)
+(*   Σ ;;; Γ ,,, Γ' ,,, Δ |- a : T -> *)
+(*   wf_local Σ (Γ ,,, subst_context s 0 Δ) -> *)
+(*   type_of Σ (Γ ,,, Γ' ,,, Δ) a = Checked T' -> *)
+(*   type_of Σ (Γ ,,, subst_context s 0 Δ) (PCUICLiftSubst.subst s #|Δ| a) = Checked (PCUICLiftSubst.subst s #|Δ| T'). *)
+(* Proof. *)
+(* Admitted. *)
+
+(* Lemma reduce_to_sort_subst: *)
+(*   forall (H : Fuel) (Σ : PCUICAst.global_context) (Γ Γ' Δ : PCUICAst.context) *)
+(*     (s : list PCUICAst.term), *)
+(*     wf Σ -> *)
+(*     subslet Σ Γ s Γ' -> *)
+(*     wf_local Σ (Γ ,,, subst_context s 0 Δ) -> *)
+(*     forall a0 : PCUICAst.term, *)
+(*       reduce_to_sort (fst Σ) (Γ ,,, subst_context s 0 Δ) (PCUICLiftSubst.subst s #|Δ| a0) = *)
+(*       reduce_to_sort (fst Σ) (Γ ,,, Γ' ,,, Δ) a0. *)
+(* Proof. *)
+(*   intros H Σ Γ Γ' Δ s X X0 X2 a0. *)
+(* Admitted. *)
+
+(* Lemma type_of_as_sort_subst Σ Γ Γ' Δ a s T : *)
+(*   wf Σ -> subslet Σ Γ s Γ' -> *)
+(*   Σ ;;; Γ ,,, Γ' ,,, Δ |- a : T -> *)
+(*   wf_local Σ (Γ ,,, subst_context s 0 Δ) -> *)
+(*   type_of_as_sort Σ (type_of Σ) (Γ ,,, subst_context s 0 Δ) *)
+(*       (PCUICLiftSubst.subst s #|Δ| a) = type_of_as_sort Σ (type_of Σ) (Γ ,,, Γ' ,,, Δ) a. *)
+(* Proof. *)
+(*   intros. unfold type_of_as_sort. *)
+(*   destruct type_of eqn:E at 2. *)
+(*   eapply type_of_subst in E; eauto. *)
+(*   - rewrite E. simpl. eapply reduce_to_sort_subst; eauto. *)
+(*   - edestruct type_of_complete; eauto. congruence. *)
+(* Qed. *)
+
+Lemma is_type_subst Σ Γ Γ' Δ a T s :
   wf Σ -> subslet Σ Γ s Γ' ->
   Σ ;;; Γ ,,, Γ' ,,, Δ |- a : T ->
   wf_local Σ (Γ ,,, subst_context s 0 Δ) ->
-  type_of Σ (Γ ,,, Γ' ,,, Δ) a = Checked T' ->
-  type_of Σ (Γ ,,, subst_context s 0 Δ) (PCUICLiftSubst.subst s #|Δ| a) = Checked (PCUICLiftSubst.subst s #|Δ| T').
-Proof.
-Admitted.
-
-Lemma reduce_to_sort_subst:
-  forall (H : Fuel) (Σ : PCUICAst.global_context) (Γ Γ' Δ : PCUICAst.context)
-    (s : list PCUICAst.term),
-    wf Σ ->
-    subslet Σ Γ s Γ' ->
-    wf_local Σ (Γ ,,, subst_context s 0 Δ) ->
-    forall a0 : PCUICAst.term,
-      reduce_to_sort (fst Σ) (Γ ,,, subst_context s 0 Δ) (PCUICLiftSubst.subst s #|Δ| a0) =
-      reduce_to_sort (fst Σ) (Γ ,,, Γ' ,,, Δ) a0.
-Proof.
-  intros H Σ Γ Γ' Δ s X X0 X2 a0.
-Admitted.
-
-Lemma type_of_as_sort_subst `{Fuel} Σ Γ Γ' Δ a s T :
-  wf Σ -> subslet Σ Γ s Γ' ->
-  Σ ;;; Γ ,,, Γ' ,,, Δ |- a : T ->
-  wf_local Σ (Γ ,,, subst_context s 0 Δ) ->
-  type_of_as_sort Σ (type_of Σ) (Γ ,,, subst_context s 0 Δ)
-      (PCUICLiftSubst.subst s #|Δ| a) = type_of_as_sort Σ (type_of Σ) (Γ ,,, Γ' ,,, Δ) a.
-Proof.
-  intros. unfold type_of_as_sort.
-  destruct type_of eqn:E at 2.
-  eapply type_of_subst in E; eauto.
-  - rewrite E. simpl. eapply reduce_to_sort_subst; eauto.
-  - edestruct type_of_complete; eauto. congruence.
-Qed.
-
-Lemma is_type_subst `{Fuel} Σ Γ Γ' Δ a T s :
-  wf Σ -> subslet Σ Γ s Γ' ->
-  Σ ;;; Γ ,,, Γ' ,,, Δ |- a : T ->
-  wf_local Σ (Γ ,,, subst_context s 0 Δ) ->
-  is_type_or_proof Σ (Γ ,,, subst_context s 0 Δ) (PCUICLiftSubst.subst s #|Δ| a) = is_type_or_proof Σ (Γ ,,, Γ' ,,, Δ) a.
+  is_type_or_proof Σ (Γ ,,, subst_context s 0 Δ) (PCUICLiftSubst.subst s #|Δ| a) = Extract.is_type_or_proof Σ (Γ ,,, Γ' ,,, Δ) a.
 Proof.
   intros.
-  unfold is_type_or_proof.
-  destruct type_of eqn:E at 2.
-  - assert (E' := E).
-    eapply type_of_sound in E' as []; eauto.
-    eapply type_of_subst in E; eauto. rewrite E. simpl.
-    destruct is_arity eqn:Ea at 2.
-    + erewrite is_arity_subst in Ea; eauto. rewrite Ea. reflexivity.
-    + erewrite is_arity_subst in Ea; eauto. rewrite Ea.
-      erewrite type_of_as_sort_subst with (Γ'0 := Γ'); eauto. admit. 
-  - edestruct type_of_complete; eauto. congruence.
+  (* unfold is_type_or_proof. *)
+  (* destruct type_of eqn:E at 2. *)
+  (* - assert (E' := E). *)
+  (*   eapply type_of_sound in E' as []; eauto. *)
+  (*   eapply type_of_subst in E; eauto. rewrite E. simpl. *)
+  (*   destruct is_arity eqn:Ea at 2. *)
+  (*   + erewrite is_arity_subst in Ea; eauto. rewrite Ea. reflexivity. *)
+  (*   + erewrite is_arity_subst in Ea; eauto. rewrite Ea. *)
+  (*     erewrite type_of_as_sort_subst with (Γ'0 := Γ'); eauto. admit.  *)
+  (* - edestruct type_of_complete; eauto. congruence. *)
 Admitted.
 
 
-Lemma extract_subst `{Fuel} Σ Γ Γ' Δ a a' s s' T :
+Lemma extract_subst Σ Γ Γ' Δ a s T :
   wf Σ ->
   subslet Σ Γ s Γ' ->
   wf_local Σ (Γ ,,, subst_context s 0 Δ) ->
   Σ ;;; Γ ,,, Γ'  ,,, Δ |- a : T ->
-  extract Σ (Γ,,,Γ',,,Δ) a = Checked a' ->
-  Forall2 (fun a b => extract Σ Γ a = Checked b) s s' ->            
-  extract Σ (Γ ,,, subst_context s 0 Δ) (PCUICLiftSubst.subst s #|Δ| a) = Checked (subst s' #|Δ| a').
+  extract Σ (Γ ,,, subst_context s 0 Δ) (PCUICLiftSubst.subst s #|Δ| a) = subst  (map (extract Σ Γ) s) #|Δ| (extract Σ (Γ,,,Γ',,,Δ) a).
 Proof.
-  intros HΣ HΔ Hs Ha.
-  pose proof (typing_wf_local Ha).
-  generalize_eqs Ha. intros eqw. rewrite <- eqw in X.
-  revert Γ Γ' Δ s Hs HΔ eqw.
-  revert Σ HΣ Γ0 X a T Ha.
-  eapply (typing_ind_env (fun Σ Γ0 a T =>
-                            forall (Γ Γ' : PCUICAst.context) Δ (s : list PCUICAst.term),
-                              wf_local Σ (Γ ,,, subst_context s 0 Δ) ->
-                              subslet Σ Γ s Γ' ->
-                              Γ0 = Γ ,,, Γ' ,,, Δ ->
-                              extract Σ (Γ ,,, Γ' ,,, Δ) a = Checked a' ->
-                              Forall2 (fun (a0 : PCUICAst.term) (b : E.term) => extract Σ Γ a0 = Checked b) s s' ->
-                              extract Σ (Γ ,,, subst_context s 0 Δ) (PCUICLiftSubst.subst s #|Δ| a) = Checked (subst s' #|Δ| a')));
-  intros Σ wfΣ Γ0 wfΓ0; intros; simpl in * |-; subst Γ0.
-  - destruct ? in H2; try congruence.
-    destruct a.
-    + inv H2. eapply is_type_extract.
-      erewrite is_type_subst; eauto.
-      econstructor; eauto.
-    + inv H2. simpl.
-      elim (leb_spec_Set); intros Hn.
-      elim nth_error_spec.
-      * intros x Heq Hlt.
-        pose proof (substlet_length X1). rewrite H1 in *.
-        rewrite -> nth_error_app_context_ge in H0 by lia.
-        rewrite -> nth_error_app_context_lt in H0 by lia.
-        eapply Forall2_nth_error_Some in H3 as (? & ? & ?); eauto.
-        rewrite H2.
-        eapply subslet_nth_error in Heq; eauto.
-         destruct decl, decl_body;
-           cbn -[skipn] in Heq.
-        -- destruct Heq as [-> ].
-           eapply (extract_weakening _ _ (subst_context s 0 Δ)) in H3; eauto.
-           rewrite subst_context_length in H3; eauto.
-        -- eapply (extract_weakening _ _ (subst_context s 0 Δ)) in H3; eauto.
-           rewrite subst_context_length in H3; eauto.
-      * intros Hs.
-        pose proof (substlet_length X1).
-        eapply Forall2_length in H3. rewrite H3 in *.
-        assert (Hs' := Hs).
-        eapply nth_error_None in Hs. rewrite Hs.
-        simpl.
-        erewrite <- is_type_subst in E; eauto.
-        cbn - [is_type_or_proof] in E.
-        revert E. elim (leb_spec_Set); intros; try lia.
-        2: econstructor; eauto.
-        rewrite <- H3 in Hs'.
-        eapply nth_error_None in Hs'.
-        rewrite Hs' in E.
-        rewrite H3 in *.
-        now rewrite E.
-      * assert (sub := X1).
-        eapply subslet_nth_error_lt in X1; eauto.
-        rewrite H0 in X1. simpl in X1.
-        simpl.
-        erewrite <- is_type_subst in E; eauto.
-        cbn - [is_type_or_proof] in E.
-        revert E. elim (leb_spec_Set); intros; try lia.
-        2: econstructor; eauto.
-        now rewrite E.
-  - 
+  (* intros HΣ HΔ Hs Ha. *)
+  (* pose proof (typing_wf_local Ha). *)
+  (* generalize_eqs Ha. intros eqw. rewrite <- eqw in X. *)
+  (* revert Γ Γ' Δ s Hs HΔ eqw. *)
+  (* revert Σ HΣ Γ0 X a T Ha. *)
+  (* eapply (typing_ind_env (fun Σ Γ0 a T => *)
+  (*                           forall (Γ Γ' : PCUICAst.context) Δ (s : list PCUICAst.term), *)
+  (*                             wf_local Σ (Γ ,,, subst_context s 0 Δ) -> *)
+  (*                             subslet Σ Γ s Γ' -> *)
+  (*                             Γ0 = Γ ,,, Γ' ,,, Δ -> *)
+  (*                             extract Σ (Γ ,,, Γ' ,,, Δ) a = Checked a' -> *)
+  (*                             Forall2 (fun (a0 : PCUICAst.term) (b : E.term) => extract Σ Γ a0 = Checked b) s s' -> *)
+  (*                             extract Σ (Γ ,,, subst_context s 0 Δ) (PCUICLiftSubst.subst s #|Δ| a) = Checked (subst s' #|Δ| a'))); *)
+  (* intros Σ wfΣ Γ0 wfΓ0; intros; simpl in * |-; subst Γ0. *)
+  (* - destruct ? in H2; try congruence. *)
+  (*   destruct a. *)
+  (*   + inv H2. eapply is_type_extract. *)
+  (*     erewrite is_type_subst; eauto. *)
+  (*     econstructor; eauto. *)
+  (*   + inv H2. simpl. *)
+  (*     elim (leb_spec_Set); intros Hn. *)
+  (*     elim nth_error_spec. *)
+  (*     * intros x Heq Hlt. *)
+  (*       pose proof (substlet_length X1). rewrite H1 in *. *)
+  (*       rewrite -> nth_error_app_context_ge in H0 by lia. *)
+  (*       rewrite -> nth_error_app_context_lt in H0 by lia. *)
+  (*       eapply Forall2_nth_error_Some in H3 as (? & ? & ?); eauto. *)
+  (*       rewrite H2. *)
+  (*       eapply subslet_nth_error in Heq; eauto. *)
+  (*        destruct decl, decl_body; *)
+  (*          cbn -[skipn] in Heq. *)
+  (*       -- destruct Heq as [-> ]. *)
+  (*          eapply (extract_weakening _ _ (subst_context s 0 Δ)) in H3; eauto. *)
+  (*          rewrite subst_context_length in H3; eauto. *)
+  (*       -- eapply (extract_weakening _ _ (subst_context s 0 Δ)) in H3; eauto. *)
+  (*          rewrite subst_context_length in H3; eauto. *)
+  (*     * intros Hs. *)
+  (*       pose proof (substlet_length X1). *)
+  (*       eapply Forall2_length in H3. rewrite H3 in *. *)
+  (*       assert (Hs' := Hs). *)
+  (*       eapply nth_error_None in Hs. rewrite Hs. *)
+  (*       simpl. *)
+  (*       erewrite <- is_type_subst in E; eauto. *)
+  (*       cbn - [is_type_or_proof] in E. *)
+  (*       revert E. elim (leb_spec_Set); intros; try lia. *)
+  (*       2: econstructor; eauto. *)
+  (*       rewrite <- H3 in Hs'. *)
+  (*       eapply nth_error_None in Hs'. *)
+  (*       rewrite Hs' in E. *)
+  (*       rewrite H3 in *. *)
+  (*       now rewrite E. *)
+  (*     * assert (sub := X1). *)
+  (*       eapply subslet_nth_error_lt in X1; eauto. *)
+  (*       rewrite H0 in X1. simpl in X1. *)
+  (*       simpl. *)
+  (*       erewrite <- is_type_subst in E; eauto. *)
+  (*       cbn - [is_type_or_proof] in E. *)
+  (*       revert E. elim (leb_spec_Set); intros; try lia. *)
+  (*       2: econstructor; eauto. *)
+  (*       now rewrite E. *)
+  (* -  *)
 Admitted.
 
-Lemma extract_subst_alt `{Fuel} Σ Γ Γ' Δ a a' s s' T :
+Lemma extract_subst_alt Σ Γ Γ' Δ a s T :
   wf Σ ->
   subslet Σ Γ s Γ' ->
   Σ ;;; Γ ,,, Γ'  ,,, Δ |- a : T ->
-  extract Σ (Γ,,,Γ',,,Δ) a = Checked a' ->
-  Forall2 (fun a b => extract Σ Γ a = Checked b) s s' ->            
-  extract Σ (Γ ,,, subst_context s 0 Δ) (PCUICLiftSubst.subst s #|Δ| a) = Checked (subst s' #|Δ| a').
+  extract Σ (Γ ,,, subst_context s 0 Δ) (PCUICLiftSubst.subst s #|Δ| a) = subst  (map (extract Σ Γ) s) #|Δ| (extract Σ (Γ,,,Γ',,,Δ) a).
 Proof.
   intros.
-  eapply extract_subst; eauto. clear H0 H1 a' H s'.
+  eapply extract_subst; eauto. (* clear H0 H1 a' H s'. *)
   eapply All_local_env_app_inv.
   apply typing_wf_local in X1; eauto.
   apply All_local_env_app in X1 as [X1 X2].
@@ -188,34 +183,30 @@ Proof.
 Qed.
 
 Lemma extract_subst1 
-      (Σ : PCUICAst.global_context) (na : name) (t b a' : PCUICAst.term) (fuel : Fuel) (a0 : E.term) T :
+      (Σ : PCUICAst.global_context) (na : name) (t b a' : PCUICAst.term) T :
   wf Σ -> Σ ;;; [] ,, PCUICAst.vass na t |- b : T -> Σ ;;; [] |- a' : t ->
-    extract Σ [PCUICAst.vass na t] b = Checked a0 ->
-    forall vea : E.term,
-      extract Σ [] a' = Checked vea -> extract Σ [] (PCUICLiftSubst.subst1 a' 0 b) = Checked (a0 {0 := vea}).
+      extract Σ [] (PCUICLiftSubst.subst1 a' 0 b) = (extract Σ [PCUICAst.vass na t] b) {0 := extract Σ [] a'}.
 Proof.
   intros HΣ Ht Hu.
   assert (wfΓ : wf_local Σ []).
   apply typing_wf_local in Hu; eauto. intros.
-  pose proof (extract_subst_alt Σ [] [PCUICAst.vass na t] [] b a0 [a'] [vea] T) as thm.
+  pose proof (extract_subst_alt Σ [] [PCUICAst.vass na t] [] b [a'] T) as thm.
   forward thm. eauto.
   forward thm. econstructor. econstructor. rewrite PCUICLiftSubst.subst_empty; auto.
   now apply (thm Ht).
 Qed.
 
 Lemma extract_subst1_vdef
-      (Σ : PCUICAst.global_context) (na : name) (t b a' : PCUICAst.term) (fuel : Fuel) (a0 : E.term) T :
-  wf Σ -> Σ ;;; [] ,, PCUICAst.vdef na a' t |- b : T ->
-    extract Σ [PCUICAst.vdef na a' t] b = Checked a0 ->
-    forall vea : E.term,
-      extract Σ [] a' = Checked vea -> extract Σ [] (PCUICLiftSubst.subst1 a' 0 b) = Checked (a0 {0 := vea}).
+      (Σ : PCUICAst.global_context) (na : name) (t b a' : PCUICAst.term) T :
+  wf Σ -> Σ ;;; [] ,, PCUICAst.vdef na a' t |- b : T -> Σ ;;; [] |- a' : t ->
+      extract Σ [] (PCUICLiftSubst.subst1 a' 0 b) = (extract Σ [PCUICAst.vdef na a' t] b) {0 := extract Σ [] a'}.
 Proof.
   intros HΣ Ht.
   assert ((wf_local Σ []) * (Σ ;;; [] |- a' : t)%type) as [wfΓ tyu].
   apply typing_wf_local in Ht; eauto with wf. 
   now depelim Ht; simpl in *; unfold PCUICAst.vdef, PCUICAst.vass in H; noconf H. 
   intros.
-  epose proof (extract_subst_alt Σ [] [PCUICAst.vdef na a' t] [] b a0 _ [vea] T HΣ) as thm.
+  epose proof (extract_subst_alt Σ [] [PCUICAst.vdef na a' t] [] b _ T HΣ) as thm.
   forward thm. econstructor. econstructor. rewrite !PCUICLiftSubst.subst_empty in *; auto.
   rewrite !PCUICLiftSubst.subst_empty in *.
   cbn in *. 
